ParserCombinators.lean
@@ -4,4 +4,5 @@ import ParserCombinators.Basic
 import ParserCombinators.Memoized
 import ParserCombinators.CFG
 import ParserCombinators.Lemmas
+import ParserCombinators.Gen
 import ParserCombinators.Example2
